Finish verification of lowerBound and contains

Orderedtree/DOrderedTree/Internal/List/Associative.lean
@@ -4,6 +4,7 @@ Released under Apache 2.0 license as described in the file LICENSE.
 Authors: Markus Himmel
 -/
 import Std.Data.DHashMap.Internal.List.Associative
+import Orderedtree.Classes.TransOrd
 
 set_option linter.missingDocs true
 set_option autoImplicit false
@@ -58,41 +59,6 @@ theorem List.min?_eq_head? {α : Type u} [Min α] {l : List α} (h : l.Pairwise 
       have hx : min x y = x := List.rel_of_pairwise_cons h (List.mem_cons_self _ _)
       rw [List.foldl_cons, ih _ (hx.symm ▸ h.sublist (by simp)), hx]
 
-theorem Ordering.eq_eq_of_isLE_of_isLE_swap {o : Ordering} : o.isLE → o.swap.isLE → o = .eq := by
-  cases o <;> simp [isLE, swap]
-
-theorem Ordering.eq_eq_of_eq_swap {o : Ordering} : o = o.swap → o = .eq := by
-  cases o <;> simp [swap]
-
-@[simp]
-theorem Ordering.isLE_eq_false {o : Ordering} : o.isLE = false ↔ o = gt := by
-  cases o <;> simp [isLE]
-
-@[simp]
-theorem Ordering.swap_eq_gt {o : Ordering} : o.swap = .gt ↔ o = .lt := by
-  cases o <;> simp [swap]
-
-theorem Ordering.isLE_iff_eq_lt_or_eq_eq {o : Ordering} : o.isLE ↔ o = .lt ∨ o = .eq := by
-  cases o <;> simp [isLE]
-
-theorem Ordering.isLE_of_eq_lt {o : Ordering} : o = .lt → o.isLE := by
-  rintro rfl; rfl
-
-theorem Ordering.isLE_of_eq_eq {o : Ordering} : o = .eq → o.isLE := by
-  rintro rfl; rfl
-
--- https://github.com/leanprover/lean4/issues/5295
-instance : LawfulBEq Ordering where
-  eq_of_beq {a b} := by cases a <;> cases b <;> simp <;> rfl
-  rfl {a} := by cases a <;> rfl
-
-theorem LawfulBEq.beq_eq_eq {α : Type u} [BEq α] [LawfulBEq α] {a b : α} : (a == b) = (a = b) := by
-  by_cases h : a = b
-  · subst h
-    simp
-  · cases h : a == b
-    · simpa
-    · simpa using eq_of_beq h
 
 variable {α : Type u} {β : α → Type v}
 
@@ -122,223 +88,46 @@ theorem getKey_beq [BEq α] {xs : List ((a : α) × β a)} {k : α} (h : contain
 
 end Std.DHashMap.Internal.List
 
-variable [Ord α]
-
 -- TODO: mark Ordering.isLE as @[inline]
 
-/-- `a == b` is defined as `compare a b == .eq`. -/
-def beqOfOrd : BEq α where
-  beq a b := compare a b == .eq
+def minSigmaOfOrd [Ord α] : Min ((a : α) × β a) where
+  min a b := if compare a.1 b.1 |>.isLE then a else b
 
-attribute [local instance] leOfOrd ltOfOrd beqOfOrd
+attribute [local instance] minSigmaOfOrd
 
-theorem le_iff {a b : α} : a ≤ b ↔ (compare a b).isLE := Iff.refl _
-theorem lt_iff {a b : α} : a < b ↔ compare a b = .lt := Iff.refl _
-theorem beq_eq {a b : α} : (a == b) = (compare a b == .eq) := rfl
-theorem beq_iff {a b : α} : (a == b) ↔ compare a b = .eq := by
-  rw [beq_eq, beq_iff_eq]
+theorem min_def [Ord α] {p q : (a : α) × β a} : min p q = if compare p.1 q.1 |>.isLE then p else q := rfl
 
-theorem le_of_lt {a b : α} : a < b → a ≤ b := by
-  rw [le_iff, lt_iff]
-  exact Ordering.isLE_of_eq_lt
-
-theorem le_iff_lt_or_beq {a b : α} : a ≤ b ↔ a < b ∨ a == b := by
-  simpa [le_iff, lt_iff, beq_iff] using Ordering.isLE_iff_eq_lt_or_eq_eq
-
-theorem le_of_beq {a b : α} (h : a == b) : a ≤ b :=
-  le_iff_lt_or_beq.2 <| Or.inr h
-
-theorem not_lt_of_beq {a b : α} : a == b → ¬a < b := by
-  simp only [beq_iff, lt_iff]
-  cases compare a b <;> simp
-
-theorem beq_eq_false_of_lt {a b : α} : a < b → (a == b) = false := by
-  simp only [beq_eq, lt_iff]
-  cases compare a b <;> simp
-
-/-- Class for "oriented" ordering functions. -/
-class OrientedOrd (α : Type u) [Ord α] where
-  /-- Swapping the arguments to `compare` swaps the result. -/
-  eq_swap {a b : α} : compare a b = (compare b a).swap
-
-theorem lt_or_lt_or_beq [OrientedOrd α] (a b : α) : a < b ∨ b < a ∨ a == b := by
-  simp only [le_iff, lt_iff, beq_eq]
-  rw [OrientedOrd.eq_swap (a := b) (b := a)]
-  cases compare a b <;> simp [Ordering.swap]
-
-@[simp]
-theorem compare_self [OrientedOrd α] {a : α} : compare a a = .eq := by
-  apply Ordering.eq_eq_of_eq_swap
-  exact OrientedOrd.eq_swap
-
-theorem compare_eq_gt_iff [OrientedOrd α] {a b : α} : compare a b = .gt ↔ compare b a = .lt := by
-  rw [OrientedOrd.eq_swap]
-  cases compare b a <;> simp
-
-theorem beq_refl [OrientedOrd α] {a : α} : a == a := by
-  simp [beq_iff]
-
-theorem beq_symm [OrientedOrd α] {a b : α} (h : a == b) : b == a := by
-  rw [beq_iff] at h
-  rw [beq_iff, OrientedOrd.eq_swap, h, Ordering.swap]
-
-theorem beq_comm [OrientedOrd α] (a b : α) : (a == b) = (b == a) := by
-  rw [beq_eq, beq_eq, OrientedOrd.eq_swap]
-  cases compare b a <;> simp [Ordering.swap, Bool.beq_eq_decide_eq]
-
-theorem irrefl [OrientedOrd α] {a b : α} : a ≤ b → b ≤ a → a == b := by
-  rw [le_iff, le_iff, beq_iff, OrientedOrd.eq_swap (a := b)]
-  exact Ordering.eq_eq_of_isLE_of_isLE_swap
-
-theorem not_lt_self [OrientedOrd α] {a : α} : ¬a < a := by
-  simp [lt_iff]
-
-theorem not_le_iff_lt [OrientedOrd α] {a b : α} : ¬a ≤ b ↔ b < a := by
-  simp [le_iff, lt_iff, OrientedOrd.eq_swap (a := a)]
-
-theorem not_lt_iff_le [OrientedOrd α] {a b : α} : ¬a < b ↔ b ≤ a :=
-  Decidable.not_iff_comm.1 not_le_iff_lt
-
-theorem not_lt_of_lt [OrientedOrd α] {a b : α} (h : a < b) : ¬b < a :=
-  not_lt_iff_le.2 (le_of_lt h)
-
-theorem lt_iff' [OrientedOrd α] {a b : α} : a < b ↔ compare b a = .gt := by
-  rw [lt_iff, compare_eq_gt_iff]
-
-/-- Class for transitive ordering functions. -/
-class TransOrd (α : Type u) [Ord α] extends OrientedOrd α where
-  /-- ≤ is transitive. -/
-  le_trans {a b c : α} : (compare a b).isLE → (compare b c).isLE → (compare a c).isLE
-
-theorem le_trans [TransOrd α] {a b c : α} : a ≤ b → b ≤ c → a ≤ c := by
-  simpa [le_iff] using TransOrd.le_trans
-
-theorem lt_of_lt_of_beq [TransOrd α] {a b c : α} (h₁ : a < b) (h₂ : b == c) : a < c := by
-  rw [← not_le_iff_lt]
-  intro h₃
-  have := not_lt_iff_le.2 (le_trans (le_of_beq h₂) h₃)
-  contradiction
-
-theorem lt_of_beq_of_lt [TransOrd α] {a b c : α} (h₁ : a == b) (h₂ : b < c) : a < c := by
-  rw [← not_le_iff_lt]
-  intro h₃
-  have := not_lt_iff_le.2 (le_trans h₃ (le_of_beq h₁))
-  contradiction
-
-theorem lt_trans [TransOrd α] {a b c : α} : a < b → b < c → a < c := by
-  intro hab hbc
-  rcases lt_or_lt_or_beq a c with (h|h|h)
-  · exact h
-  · have := not_lt_iff_le.2 (le_trans (le_of_lt hbc) (le_of_lt h))
-    contradiction
-  · have := not_lt_iff_le.2 (le_of_lt (lt_of_lt_of_beq hbc (beq_symm h)))
-    contradiction
-
-theorem beq_trans [TransOrd α] {a b c : α} (h₁ : a == b) (h₂ : b == c) : a == c := by
-  rcases lt_or_lt_or_beq a c with (h|h|h)
-  · rw [beq_eq_false_of_lt (lt_of_lt_of_beq h (beq_symm h₂))] at h₁
-    contradiction
-  · rw [beq_comm, beq_eq_false_of_lt (lt_of_beq_of_lt h₂ h)] at h₁
-    contradiction
-  · exact h
-
-local instance equivBEqOfTransOrd [TransOrd α] : EquivBEq α where
-  symm := beq_symm
-  trans := beq_trans
-  refl := beq_refl
-
-theorem lt_of_le_of_lt [TransOrd α] {a b c : α} : a ≤ b → b < c → a < c := by
-  intros hab hbc
-  rcases le_iff_lt_or_beq.1 hab with (hab|hab)
-  · exact lt_trans hab hbc
-  . exact lt_of_beq_of_lt hab hbc
-
-theorem lt_of_lt_of_le [TransOrd α] {a b c : α} : a < b → b ≤ c → a < c := by
-  intros hab hbc
-  rcases le_iff_lt_or_beq.1 hbc with (hbc|hbc)
-  · exact lt_trans hab hbc
-  · exact lt_of_lt_of_beq hab hbc
-
-
--- local instance : Min α where
---   min a b := if a ≤ b then a else b
-
--- theorem min_def {a b : α} : min a b = if a ≤ b then a else b := rfl
-
--- -- Is this provable without `TransOrd`?
--- local instance [TransOrd α] : Std.Associative (min : α → α → α) where
---   assoc a b c := by
---     simp only [min_def]
---     split <;> split <;> (try split) <;> try rfl
---     · rename_i hab hac hbc
---       have := le_trans hab hbc
---       contradiction
---     · rename_i hab hbc hac
---       rw [not_le_iff_lt] at hab hbc
---       have := lt_trans hbc hab
---       rw [← not_lt_iff_le] at hac
---       contradiction
-
-local instance : Min ((a : α) × β a) where
-  min a b := if a.1 ≤ b.1 then a else b
-
-theorem min_def' {p q : (a : α) × β a} : min p q = if p.1 ≤ q.1 then p else q := rfl
-
-theorem min_eq_or {p q : (a : α) × β a} : min p q = p ∨ min p q = q := by
-  rw [min_def']
+theorem min_eq_or [Ord α] {p q : (a : α) × β a} : min p q = p ∨ min p q = q := by
+  rw [min_def]
   split <;> simp
 
-theorem min_eq_left' {p q : (a : α) × β a} (h : p.1 ≤ q.1) : min p q = p := by
-  simp [min_def', h]
+theorem min_eq_left [Ord α] {p q : (a : α) × β a} (h : compare p.1 q.1 |>.isLE) : min p q = p := by
+  simp [min_def, h]
 
-theorem min_eq_left_of_lt' {p q : (a : α) × β a} (h : p.1 < q.1) : min p q = p :=
-  min_eq_left' (le_of_lt h)
+theorem min_eq_left_of_lt [Ord α] {p q : (a : α) × β a} (h : compare p.1 q.1 = .lt) : min p q = p :=
+  min_eq_left (Ordering.isLE_of_eq_lt h)
 
 -- Is this provable without `TransOrd`?
-local instance [TransOrd α] : Std.Associative (min : (a : α) × β a → (a : α) × β a → (a : α) × β a) where
+local instance [Ord α] [TransOrd α] : Std.Associative (min : (a : α) × β a → (a : α) × β a → (a : α) × β a) where
   assoc a b c := by
-    simp only [min_def']
+    simp only [min_def]
     split <;> split <;> (try split) <;> try rfl
     · rename_i hab hac hbc
-      have := le_trans hab hbc
+      have := TransCmp.le_trans hab hbc
       contradiction
     · rename_i hab hbc hac
-      rw [not_le_iff_lt] at hab hbc
-      have := lt_trans hbc hab
-      rw [← not_lt_iff_le] at hac
-      contradiction
+      simp only [Bool.not_eq_true, Ordering.isLE_eq_false] at hab hbc
+      refine absurd hac ?_
+      simp only [Bool.not_eq_true, Ordering.isLE_eq_false]
+      exact OrientedCmp.gt_of_lt (TransCmp.lt_trans (OrientedCmp.lt_of_gt hbc) (OrientedCmp.lt_of_gt hab))
 
 namespace Std.DHashMap.Internal.List
 
-theorem eq_append [TransOrd α] {l : List ((a : α) × β a)} (hl : l.Pairwise (·.1 < ·.1)) {k : α} :
-    l = l.filter (·.1 < k) ++ ((l.find? (·.1 == k)).toList ++ l.filter (k < ·.1)) := by
-  induction l with
-  | nil => simp
-  | cons x l ih =>
-    rcases lt_or_lt_or_beq x.1 k with hx|hx|hx
-    · simpa [List.filter_cons, hx, not_lt_of_lt hx, List.find?_cons, beq_eq_false_of_lt hx] using ih hl.of_cons
-    · have h₁ (y) (hy : y ∈ l) : ¬(decide (y.1 < k)) = true := by
-        simp only [decide_eq_true_eq]
-        exact not_lt_of_lt (lt_trans hx (List.rel_of_pairwise_cons hl hy))
-      have h₂ (y) (hy : y ∈ l) : ¬(y.1 == k) = true := by
-        simp only [Bool.not_eq_true]
-        exact BEq.symm_false (beq_eq_false_of_lt (lt_trans hx (List.rel_of_pairwise_cons hl hy)))
-      simpa [List.filter_cons, hx, not_lt_of_lt hx, List.find?_cons, BEq.symm_false (beq_eq_false_of_lt hx),
-        List.filter_eq_nil_iff.2 h₁, List.find?_eq_none.2 h₂] using ih hl.of_cons
-    · have h₁ (y) (hy : y ∈ l) : ¬(decide (y.1 < k)) = true := by
-        simp only [decide_eq_true_eq]
-        exact not_lt_of_lt (lt_of_beq_of_lt (BEq.symm hx) (List.rel_of_pairwise_cons hl hy))
-      have h₂ (y) (hy : y ∈ l) : ¬(y.1 == k) = true := by
-        simp only [Bool.not_eq_true]
-        refine BEq.symm_false (beq_eq_false_of_lt (lt_of_beq_of_lt (BEq.symm hx) (List.rel_of_pairwise_cons hl hy)))
-      simpa [List.filter_cons, List.filter_eq_nil_iff.2 h₁, not_lt_of_beq hx, not_lt_of_beq (BEq.symm hx),
-        List.find?_cons, hx, List.find?_eq_none.2 h₂] using ih hl.of_cons
-
 /-- The smallest element of `xs` that is not less than `k`. -/
-def lowerBound? (xs : List ((a : α) × β a)) (k : α) : Option ((a : α) × β a) :=
-  xs.filter (fun p => k ≤ p.1) |>.min?
+def lowerBound? [Ord α] (k : α) (xs : List ((a : α) × β a)) : Option ((a : α) × β a) :=
+  xs.filter (fun p => compare k p.1 |>.isLE) |>.min?
 
-theorem lowerBound?_mem {xs : List ((a : α) × β a)} {k : α} {p : (a : α) × β a} (h : lowerBound? xs k = some p) :
+theorem lowerBound?_mem [Ord α] {xs : List ((a : α) × β a)} {k : α} {p : (a : α) × β a} (h : lowerBound? k xs = some p) :
     p ∈ xs := by
   rw [lowerBound?] at h
   have := List.min?_mem (@min_eq_or _ _ _) h
@@ -346,112 +135,114 @@ theorem lowerBound?_mem {xs : List ((a : α) × β a)} {k : α} {p : (a : α) ×
   exact this.1
 
 /-- The smallest element of `xs` that is greater than `k`. -/
-def upperBound? (xs : List ((a : α) × β a)) (k : α) : Option ((a : α) × β a) :=
-  xs.filter (fun p => p.1 < k) |>.min?
+def upperBound? [Ord α] (xs : List ((a : α) × β a)) (k : α) : Option ((a : α) × β a) :=
+  xs.filter (fun p => compare k p.1 = .lt) |>.min?
 
 @[simp]
-theorem lowerBound?_nil {k : α} : lowerBound? ([] : List ((a : α) × β a)) k = none := rfl
+theorem lowerBound?_nil [Ord α] {k : α} : lowerBound? k ([] : List ((a : α) × β a)) = none := rfl
 
-theorem lowerBound?_cons [TransOrd α] (l : List ((a : α) × β a)) (k : α) (v : β k) (a : α) :
-    lowerBound? (⟨k, v⟩ :: l) a =
-      if k < a then lowerBound? l a else some ((lowerBound? l a).elim ⟨k, v⟩ (min ⟨k, v⟩)) := by
-  rw [lowerBound?, List.filter_cons]
-  simp only [decide_eq_true_eq]
-  split
-  · rw [List.min?_cons]
-    split
-    · exact False.elim (not_lt_self (lt_of_le_of_lt (b := k) ‹_› ‹_›))
-    · rfl
-  · next h =>
-    rw [not_le_iff_lt] at h
-    simp [h, lowerBound?]
+-- theorem lowerBound?_cons [Ord α] [TransOrd α] (l : List ((a : α) × β a)) (k : α) (v : β k) (a : α) :
+--     lowerBound? (⟨k, v⟩ :: l) a =
+--       if compare k a = .lt then lowerBound? l a else some ((lowerBound? l a).elim ⟨k, v⟩ (min ⟨k, v⟩)) := by
+--   rw [lowerBound?, List.filter_cons]
+--   simp only [decide_eq_true_eq]
+--   split
+--   · rw [List.min?_cons]
+--     split
+--     · exact False.elim (not_lt_self (lt_of_le_of_lt (b := k) ‹_› ‹_›))
+--     · rfl
+--   · next h =>
+--     rw [not_le_iff_lt] at h
+--     simp [h, lowerBound?]
 
-theorem lowerBound?_cons_eq_self [TransOrd α] {l : List ((a : α) × β a)} {p : (a : α) × β a} {k : α}
-    (hp : k ≤ p.1) (hl : ∀ q ∈ l, q.1 < k ∨ p.1 ≤ q.1) : lowerBound? (p :: l) k = some p := by
-  rw [lowerBound?_cons]
-  simp only [not_lt_iff_le.2 hp, ↓reduceIte, Option.some.injEq]
-  rw [lowerBound?]
-  cases h : (l.filter (fun p => k ≤ p.1)).min? with
-  | none => simp
-  | some q =>
-    have := List.mem_filter.1 (List.min?_mem (fun _ _ => min_eq_or) h)
-    simp only [decide_eq_true_eq] at this
-    suffices p.1 ≤ q.1 by simpa using min_eq_left' this
-    exact (hl _ this.1).resolve_left (not_lt_iff_le.2 this.2)
+-- theorem lowerBound?_cons_eq_self [TransOrd α] {l : List ((a : α) × β a)} {p : (a : α) × β a} {k : α}
+--     (hp : k ≤ p.1) (hl : ∀ q ∈ l, q.1 < k ∨ p.1 ≤ q.1) : lowerBound? (p :: l) k = some p := by
+--   rw [lowerBound?_cons]
+--   simp only [not_lt_iff_le.2 hp, ↓reduceIte, Option.some.injEq]
+--   rw [lowerBound?]
+--   cases h : (l.filter (fun p => k ≤ p.1)).min? with
+--   | none => simp
+--   | some q =>
+--     have := List.mem_filter.1 (List.min?_mem (fun _ _ => min_eq_or) h)
+--     simp only [decide_eq_true_eq] at this
+--     suffices p.1 ≤ q.1 by simpa using min_eq_left' this
+--     exact (hl _ this.1).resolve_left (not_lt_iff_le.2 this.2)
 
-theorem min_comm_of_lt_or_lt [OrientedOrd α] {p p' : (a : α) × β a} (h : p.1 < p'.1 ∨ p'.1 < p.1) :
-    min p p' = min p' p := by
-  rcases h with h|h <;> simp [min_def', le_of_lt h, not_le_iff_lt.2 h]
+-- theorem min_comm_of_lt_or_lt [OrientedOrd α] {p p' : (a : α) × β a} (h : p.1 < p'.1 ∨ p'.1 < p.1) :
+--     min p p' = min p' p := by
+--   rcases h with h|h <;> simp [min_def', le_of_lt h, not_le_iff_lt.2 h]
 
-theorem lt_or_lt_of_containsKey_eq_false [TransOrd α] {l : List ((a : α) × β a)} {p : (a : α) × β a} {k : α}
-    (hp : p ∈ l) (hk : containsKey k l = false) : p.1 < k ∨ k < p.1 := by
-  rcases lt_or_lt_or_beq p.1 k with h|h|h
-  · exact Or.inl h
-  · exact Or.inr h
-  · rw [containsKey_congr (BEq.symm h), containsKey_of_mem hp] at hk
-    contradiction
+-- theorem lt_or_lt_of_containsKey_eq_false [TransOrd α] {l : List ((a : α) × β a)} {p : (a : α) × β a} {k : α}
+--     (hp : p ∈ l) (hk : containsKey k l = false) : p.1 < k ∨ k < p.1 := by
+--   rcases lt_or_lt_or_beq p.1 k with h|h|h
+--   · exact Or.inl h
+--   · exact Or.inr h
+--   · rw [containsKey_congr (BEq.symm h), containsKey_of_mem hp] at hk
+--     contradiction
 
-theorem lowerBound?_of_perm [TransOrd α] {l l' : List ((a : α) × β a)} (hll' : List.Perm l l') {k : α} (hl : DistinctKeys l) :
-    lowerBound? l k = lowerBound? l' k := by
-  induction hll' with
-  | nil => rfl
-  | @cons x l l' _ ih => rw [lowerBound?_cons, lowerBound?_cons, ih hl.tail]
-  | swap x y l =>
-    rw [lowerBound?_cons, lowerBound?_cons, lowerBound?_cons, lowerBound?_cons]
-    split <;> split <;> try (simp; done)
-    rename_i hyk hxk
-    have hxy : x.1 < y.1 ∨ y.1 < x.1 :=
-      lt_or_lt_of_containsKey_eq_false (List.mem_cons_self _ _) hl.containsKey_eq_false
-    cases lowerBound? l k with
-    | none => simpa using (min_comm_of_lt_or_lt hxy).symm
-    | some p => simp [← Std.Associative.assoc (op := min), min_comm_of_lt_or_lt hxy]
-  | trans h₁ _ ih₁ ih₂ => rw [ih₁ hl, ih₂ (hl.perm h₁.symm)]
+-- theorem lowerBound?_of_perm [TransOrd α] {l l' : List ((a : α) × β a)} (hll' : List.Perm l l') {k : α} (hl : DistinctKeys l) :
+--     lowerBound? l k = lowerBound? l' k := by
+--   induction hll' with
+--   | nil => rfl
+--   | @cons x l l' _ ih => rw [lowerBound?_cons, lowerBound?_cons, ih hl.tail]
+--   | swap x y l =>
+--     rw [lowerBound?_cons, lowerBound?_cons, lowerBound?_cons, lowerBound?_cons]
+--     split <;> split <;> try (simp; done)
+--     rename_i hyk hxk
+--     have hxy : x.1 < y.1 ∨ y.1 < x.1 :=
+--       lt_or_lt_of_containsKey_eq_false (List.mem_cons_self _ _) hl.containsKey_eq_false
+--     cases lowerBound? l k with
+--     | none => simpa using (min_comm_of_lt_or_lt hxy).symm
+--     | some p => simp [← Std.Associative.assoc (op := min), min_comm_of_lt_or_lt hxy]
+--   | trans h₁ _ ih₁ ih₂ => rw [ih₁ hl, ih₂ (hl.perm h₁.symm)]
 
-theorem lowerBound?_replaceEntry_cons_of_beq [TransOrd α] {l : List ((a : α) × β a)}
-    {k a : α} {v : β k} {p : (a : α) × β a} (h : p.1 == k) : lowerBound? (replaceEntry k v (p :: l)) a =
-      if k < a then lowerBound? l a else some ((lowerBound? l a).elim ⟨k, v⟩ (min ⟨k, v⟩)) := by
-  rw [replaceEntry_cons_of_true h, lowerBound?_cons]
+-- theorem lowerBound?_replaceEntry_cons_of_beq [TransOrd α] {l : List ((a : α) × β a)}
+--     {k a : α} {v : β k} {p : (a : α) × β a} (h : p.1 == k) : lowerBound? (replaceEntry k v (p :: l)) a =
+--       if k < a then lowerBound? l a else some ((lowerBound? l a).elim ⟨k, v⟩ (min ⟨k, v⟩)) := by
+--   rw [replaceEntry_cons_of_true h, lowerBound?_cons]
 
-theorem lowerBound?_replaceEntry_of_containsKey_eq_true [TransOrd α] {l : List ((a : α) × β a)}
-      {k : α} {v : β k} {a : α} (h : containsKey k l) (hl : DistinctKeys l) :
-    lowerBound? (replaceEntry k v l) a = if k < a then lowerBound? l a else some ((lowerBound? l a).elim ⟨k, v⟩ (min ⟨k, v⟩)) := by
-  obtain ⟨l', hl'⟩ := perm_cons_getEntry h
-  rw [lowerBound?_of_perm (replaceEntry_of_perm hl hl') hl.replaceEntry]
-  rw [lowerBound?_replaceEntry_cons_of_beq (by simpa using getKey_beq _)]
-  rw [lowerBound?_of_perm hl' hl, lowerBound?_cons]
-  split <;> split
-  · rfl
-  · rename_i h₁ h₂
-    simp only [getEntry_fst] at h₂
-    have h₁' := lt_of_beq_of_lt (getKey_beq h) h₁
-    contradiction
-  · simp
-  · have hk : k ≤ getKey k l h := le_of_beq (BEq.symm (getKey_beq h))
-    cases lowerBound? l' a with
-    | none => simp [min_def', hk]
-    | some p =>
-      simp only [Option.elim_some, Option.some.injEq]
-      rw [← Std.Associative.assoc (op := min)]
-      congr 1
-      simp [min_def', hk]
+-- theorem lowerBound?_replaceEntry_of_containsKey_eq_true [TransOrd α] {l : List ((a : α) × β a)}
+--       {k : α} {v : β k} {a : α} (h : containsKey k l) (hl : DistinctKeys l) :
+--     lowerBound? (replaceEntry k v l) a = if k < a then lowerBound? l a else some ((lowerBound? l a).elim ⟨k, v⟩ (min ⟨k, v⟩)) := by
+--   obtain ⟨l', hl'⟩ := perm_cons_getEntry h
+--   rw [lowerBound?_of_perm (replaceEntry_of_perm hl hl') hl.replaceEntry]
+--   rw [lowerBound?_replaceEntry_cons_of_beq (by simpa using getKey_beq _)]
+--   rw [lowerBound?_of_perm hl' hl, lowerBound?_cons]
+--   split <;> split
+--   · rfl
+--   · rename_i h₁ h₂
+--     simp only [getEntry_fst] at h₂
+--     have h₁' := lt_of_beq_of_lt (getKey_beq h) h₁
+--     contradiction
+--   · simp
+--   · have hk : k ≤ getKey k l h := le_of_beq (BEq.symm (getKey_beq h))
+--     cases lowerBound? l' a with
+--     | none => simp [min_def', hk]
+--     | some p =>
+--       simp only [Option.elim_some, Option.some.injEq]
+--       rw [← Std.Associative.assoc (op := min)]
+--       congr 1
+--       simp [min_def', hk]
 
-theorem lowerBound?_insertEntry [TransOrd α] (xs : List ((a : α) × β a)) (k : α) (v : β k) (a : α) (h : DistinctKeys xs) :
-    lowerBound? (insertEntry k v xs) a =
-      if k < a then lowerBound? xs a else some ((lowerBound? xs a).elim ⟨k, v⟩ (min ⟨k, v⟩)) := by
-  rw [insertEntry]
-  cases hc : containsKey k xs
-  · rw [cond_false, lowerBound?_cons]
-  · rw [cond_true, lowerBound?_replaceEntry_of_containsKey_eq_true hc h]
+-- theorem lowerBound?_insertEntry [TransOrd α] (xs : List ((a : α) × β a)) (k : α) (v : β k) (a : α) (h : DistinctKeys xs) :
+--     lowerBound? (insertEntry k v xs) a =
+--       if k < a then lowerBound? xs a else some ((lowerBound? xs a).elim ⟨k, v⟩ (min ⟨k, v⟩)) := by
+--   rw [insertEntry]
+--   cases hc : containsKey k xs
+--   · rw [cond_false, lowerBound?_cons]
+--   · rw [cond_true, lowerBound?_replaceEntry_of_containsKey_eq_true hc h]
 
-theorem lowerBound?_append_of_forall_mem_left [TransOrd α] {l₁ l₂ : List ((a : α) × β a)} {k : α} (h : ∀ p ∈ l₁, p.1 < k) :
-    lowerBound? (l₁ ++ l₂) k = lowerBound? l₂ k := by
+theorem lowerBound?_append_of_forall_mem_left [Ord α] [TransOrd α] {l₁ l₂ : List ((a : α) × β a)}
+    {k : α} (h : ∀ p ∈ l₁, compare k p.1 = .gt) :
+    lowerBound? k (l₁ ++ l₂) = lowerBound? k l₂ := by
   rw [lowerBound?, lowerBound?, List.filter_append, List.filter_eq_nil_iff.2, List.nil_append]
-  exact fun p hp => by simpa using not_le_iff_lt.2 (h p hp)
+  refine fun p hp => by simpa using h p hp
 
-theorem lowerBound?_eq_head? {l : List ((a : α) × β a)} {k : α} (h : ∀ p ∈ l, k ≤ p.1) (hl : l.Pairwise (fun a b => a.1 < b.1)) :
-    lowerBound? l k = l.head? := by
-  rw [lowerBound?, List.filter_eq_self.2 (decide_eq_true <| h · ·), List.min?_eq_head? (hl.imp min_eq_left_of_lt')]
+theorem lowerBound?_eq_head? [Ord α] {l : List ((a : α) × β a)} {k : α} (h : ∀ p ∈ l, compare k p.1 |>.isLE)
+    (hl : l.Pairwise (fun a b => compare a.1 b.1 = .lt)) : lowerBound? k l = l.head? := by
+  rw [lowerBound?, List.filter_eq_self.2 h, List.min?_eq_head? (hl.imp min_eq_left_of_lt)]
 
+/-
 /-- The number of entries whose key is strictly less than the given key. -/
 def rank (k : α) (l : List ((a : α) × β a)) : Nat :=
   l.filter (·.1 < k) |>.length
@@ -462,6 +253,6 @@ theorem rank_append_eq_left [OrientedOrd α] {k : α} {l₁ l₂ : List ((a : α
 
 theorem rank_eq_length {k : α} {l : List ((a : α) × β a)} (hl : ∀ p ∈ l, p.1 < k) :
     rank k l = l.length := by
-  simpa [rank]
+  simpa [rank]-/
 
 end Std.DHashMap.Internal.List
